aarch64 infoflow: prove noninterference
Signed-off-by: Ryan Barry <ryan.barry@proofcraft.systems>

proof/infoflow/AARCH64/ArchCNode_IF.thy
@@ -8,7 +8,7 @@ theory ArchCNode_IF
 imports CNode_IF
 begin
 
-context Arch begin global_naming AARCH64
+context Arch begin arch_global_naming
 
 named_theorems CNode_IF_assms
 
@@ -28,48 +28,19 @@ lemma set_object_globals_equiv:
   apply (clarsimp simp: globals_equiv_def idle_equiv_def tcb_at_def2)
   done
 
-lemma set_object_globals_equiv'':
-  "\<lbrace>globals_equiv s and (\<lambda> s. ptr \<noteq> arm_us_global_vspace (arch_state s)) and (\<lambda>t. ptr \<noteq> idle_thread t)\<rbrace>
-   set_object ptr obj
-   \<lbrace>\<lambda>_. globals_equiv s\<rbrace>"
-  by (wpsimp wp: set_object_globals_equiv)
-
-lemma set_cap_globals_equiv':
-  "\<lbrace>globals_equiv s and (\<lambda> s. fst p \<noteq> arm_us_global_vspace (arch_state s))\<rbrace>
-   set_cap cap p
-   \<lbrace>\<lambda>_. globals_equiv s\<rbrace>"
-  unfolding set_cap_def
-  apply (simp only: split_def)
-  apply (wp set_object_globals_equiv hoare_vcg_all_lift get_object_wp | wpc | simp)+
-  apply (fastforce simp: obj_at_def is_tcb_def)
-  done
-
 lemma set_cap_globals_equiv[CNode_IF_assms]:
-  "\<lbrace>globals_equiv s and valid_global_objs and valid_arch_state\<rbrace>
+  "\<lbrace>globals_equiv s and valid_arch_state\<rbrace>
    set_cap cap p
    \<lbrace>\<lambda>_. globals_equiv s\<rbrace>"
   unfolding set_cap_def
   apply (simp only: split_def)
   apply (wp set_object_globals_equiv hoare_vcg_all_lift get_object_wp | wpc | simp)+
-  apply (fastforce simp: is_tcb_def obj_at_def valid_arch_state_def
-                   dest: valid_global_arch_objs_pt_at)
+  apply (fastforce simp: valid_arch_state_def obj_at_def is_tcb_def
+                   dest: valid_global_arch_objs_pt_at)+
   done
 
 definition irq_at :: "nat \<Rightarrow> (irq \<Rightarrow> bool) \<Rightarrow> irq option" where
-  "irq_at pos masks \<equiv> let i = irq_oracle pos in (if i = 0x3F \<or> masks i then None else Some i)"
-
-lemma dmo_getActiveIRQ_wp[CNode_IF_assms]:
-  "\<lbrace>\<lambda>s. P (irq_at (irq_state (machine_state s) + 1) (irq_masks (machine_state s)))
-          (s\<lparr>machine_state := (machine_state s\<lparr>irq_state := irq_state (machine_state s) + 1\<rparr>)\<rparr>)\<rbrace>
-   do_machine_op (getActiveIRQ in_kernel)
-   \<lbrace>P\<rbrace>"
-  apply (simp add: do_machine_op_def getActiveIRQ_def non_kernel_IRQs_def)
-  apply (wp modify_wp | wpc)+
-  apply clarsimp
-  apply (erule use_valid)
-   apply (wp modify_wp)
-  apply (auto simp: irq_at_def Let_def split: if_splits)
-  done
+  "irq_at pos masks \<equiv> let i = irq_oracle pos in (if masks i then None else Some i)"
 
 lemma arch_globals_equiv_irq_state_update[CNode_IF_assms, simp]:
   "arch_globals_equiv ct it kh kh' as as' ms (irq_state_update f ms') =
@@ -81,7 +52,7 @@ lemma arch_globals_equiv_irq_state_update[CNode_IF_assms, simp]:
 end
 
 
-requalify_consts AARCH64.irq_at
+arch_requalify_consts irq_at
 
 global_interpretation CNode_IF_1?: CNode_IF_1 _ irq_at
 proof goal_cases
@@ -91,7 +62,7 @@ proof goal_cases
 qed
 
 
-context Arch begin global_naming AARCH64
+context Arch begin arch_global_naming
 
 lemma is_irq_at_triv[CNode_IF_assms]:
   assumes a: "\<And>P. \<lbrace>(\<lambda>s. P (irq_masks (machine_state s))) and Q\<rbrace>
@@ -118,20 +89,29 @@ proof goal_cases
 qed
 
 
-context Arch begin global_naming AARCH64
+context Arch begin arch_global_naming
 
 lemma dmo_getActiveIRQ_reads_respects[CNode_IF_assms]:
   notes gets_ev[wp del]
   shows "reads_respects aag l (invs and only_timer_irq_inv irq st)
                        (do_machine_op (getActiveIRQ in_kernel))"
-  apply (rule use_spec_ev)
-  apply (rule do_machine_op_spec_reads_respects')
+  apply (rule do_machine_op_reads_respects')
    apply (simp add: getActiveIRQ_def)
    apply (wp irq_state_increment_reads_respects_memory irq_state_increment_reads_respects_device
              gets_ev[where f="irq_oracle \<circ> irq_state"] equiv_valid_inv_conj_lift
              gets_irq_masks_equiv_valid modify_wp
           | simp add: no_irq_def)+
   apply (rule only_timer_irq_inv_determines_irq_masks, blast+)
+   apply (wpsimp simp: irq_state_independent_def)+
+  done
+
+lemma dmo_getActiveIRQ_globals_equiv[CNode_IF_assms]:
+  "do_machine_op (getActiveIRQ in_kernel) \<lbrace>globals_equiv st\<rbrace>"
+  unfolding globals_equiv_def arch_globals_equiv_def idle_equiv_def
+  apply (rule hoare_weaken_pre)
+   apply wps
+   apply wpsimp
+  apply clarsimp
   done
 
 end
