proof/infoflow/AARCH64/ArchInfoFlow_IF.thy
@@ -8,9 +8,23 @@ theory ArchInfoFlow_IF
 imports InfoFlow_IF
 begin
 
-context Arch begin global_naming AARCH64
+context Arch begin arch_global_naming
 
 named_theorems InfoFlow_IF_assms
+
+definition identical_hyp_state_updates ::
+  "(obj_ref \<Rightarrow> bool) \<Rightarrow> det_state \<Rightarrow> det_state \<Rightarrow> machine_state \<Rightarrow> machine_state \<Rightarrow> bool" where
+  "identical_hyp_state_updates P s s' ms ms' \<equiv>
+     identical_updates_for P (hw_vcpu_of s) (hw_vcpu_of s')
+                             (hw_vcpu_of (s\<lparr>machine_state := ms\<rparr>))
+                             (hw_vcpu_of (s'\<lparr>machine_state := ms'\<rparr>))"
+
+definition identical_fpu_state_updates ::
+  "(obj_ref \<Rightarrow> bool) \<Rightarrow> det_state \<Rightarrow> det_state \<Rightarrow> machine_state \<Rightarrow> machine_state \<Rightarrow> bool" where
+  "identical_fpu_state_updates P s s' ms ms' \<equiv>
+     identical_updates_for P (hw_fpu_of s) (hw_fpu_of s')
+                             (hw_fpu_of (s\<lparr>machine_state := ms\<rparr>))
+                             (hw_fpu_of (s'\<lparr>machine_state := ms'\<rparr>))"
 
 lemma asid_pool_at_kheap:
   "asid_pool_at ptr s = (\<exists>asid_pool. kheap s ptr = Some (ArchObj (ASIDPool asid_pool)))"
@@ -34,6 +48,10 @@ lemma equiv_asids_trans[InfoFlow_IF_assms]:
   "\<lbrakk> equiv_asids R s t; equiv_asids R t u \<rbrakk> \<Longrightarrow> equiv_asids R s u"
   by (fastforce simp: equiv_asids_def equiv_asid_def asid_pool_at_kheap asid_pools_of_ko_at obj_at_def)
 
+lemma equiv_asids_guard_imp[InfoFlow_IF_assms]:
+  "\<lbrakk> equiv_asids R s s'; \<And>x. Q x \<Longrightarrow> R x \<rbrakk> \<Longrightarrow> equiv_asids Q s s'"
+  by (auto simp: equiv_asids_def)
+
 lemma equiv_asids_non_asid_pool_kheap_update[InfoFlow_IF_assms]:
   "\<lbrakk> equiv_asids R s s'; non_asid_pool_kheap_update s kh; non_asid_pool_kheap_update s' kh' \<rbrakk>
      \<Longrightarrow> equiv_asids R (s\<lparr>kheap := kh\<rparr>) (s'\<lparr>kheap := kh'\<rparr>)"
@@ -49,10 +67,6 @@ lemma equiv_asids_identical_kheap_updates[InfoFlow_IF_assms]:
   apply (case_tac "kh pool_ptr = kh' pool_ptr"; fastforce)
   done
 
-lemma equiv_asids_trivial[InfoFlow_IF_assms]:
-  "(\<And>x. P x \<Longrightarrow> False) \<Longrightarrow> equiv_asids P x y"
-  by (auto simp: equiv_asids_def)
-
 lemma equiv_asids_triv':
   "\<lbrakk> equiv_asids R s s'; kheap t = kheap s; kheap t' = kheap s';
      arm_asid_table (arch_state t) = arm_asid_table (arch_state s);
@@ -65,6 +79,80 @@ lemma equiv_asids_triv[InfoFlow_IF_assms]:
      arch_state t = arch_state s; arch_state t' = arch_state s' \<rbrakk>
      \<Longrightarrow> equiv_asids R t t'"
   by (fastforce simp: equiv_asids_triv')
+
+lemma equiv_hyp_refl[InfoFlow_IF_assms]:
+  "equiv_hyp P s s"
+  by (auto simp: equiv_hyp_def equiv_for_def)
+
+lemma equiv_hyp_sym[InfoFlow_IF_assms]:
+  "equiv_hyp P s t \<Longrightarrow> equiv_hyp P t s"
+  by (auto simp: equiv_hyp_def equiv_for_def)
+
+lemma equiv_hyp_trans[InfoFlow_IF_assms]:
+  "\<lbrakk> equiv_hyp P s t; equiv_hyp P t u \<rbrakk> \<Longrightarrow> equiv_hyp P s u"
+  by (fastforce simp: equiv_hyp_def equiv_for_def)
+
+lemma equiv_hyp_guard_imp[InfoFlow_IF_assms]:
+  "\<lbrakk> equiv_hyp P s s'; \<And>x. Q x \<Longrightarrow> P x \<rbrakk> \<Longrightarrow> equiv_hyp Q s s'"
+  by (fastforce simp: equiv_hyp_def equiv_for_def)
+
+lemma equiv_hyp_triv':
+  "\<lbrakk> equiv_hyp P s s';
+     arm_current_vcpu (arch_state t) = arm_current_vcpu (arch_state s);
+     arm_current_vcpu (arch_state t') = arm_current_vcpu (arch_state s');
+     vcpu_state (machine_state t) = vcpu_state (machine_state s);
+     vcpu_state (machine_state t') = vcpu_state (machine_state s');
+     arm_gicvcpu_numlistregs (arch_state t) = arm_gicvcpu_numlistregs (arch_state s);
+     arm_gicvcpu_numlistregs (arch_state t') = arm_gicvcpu_numlistregs (arch_state s') \<rbrakk>
+     \<Longrightarrow> equiv_hyp P t t'"
+  by (fastforce simp: equiv_hyp_def equiv_for_def)
+
+lemma equiv_hyp_triv[InfoFlow_IF_assms]:
+  "\<lbrakk> equiv_hyp P s s'; arch_state t = arch_state s; arch_state t' = arch_state s';
+     machine_state t = machine_state s; machine_state t' = machine_state s' \<rbrakk>
+     \<Longrightarrow> equiv_hyp P t t'"
+  by (fastforce simp: equiv_hyp_triv')
+
+lemma equiv_hyp_machine_state_update[InfoFlow_IF_assms]:
+  "\<lbrakk> equiv_hyp P s s'; identical_hyp_state_updates P s s' ms ms' \<rbrakk>
+     \<Longrightarrow> equiv_hyp P (s\<lparr>machine_state := ms\<rparr>) (s'\<lparr>machine_state := ms'\<rparr>)"
+  by (fastforce simp: equiv_hyp_def equiv_for_def identical_hyp_state_updates_def identical_updates_def)
+
+lemma equiv_fpu_refl[InfoFlow_IF_assms]:
+  "equiv_fpu P s s"
+  by (auto simp: equiv_fpu_def equiv_for_def)
+
+lemma equiv_fpu_sym[InfoFlow_IF_assms]:
+  "equiv_fpu P s t \<Longrightarrow> equiv_fpu P t s"
+  by (auto simp: equiv_fpu_def equiv_for_def)
+
+lemma equiv_fpu_trans[InfoFlow_IF_assms]:
+  "\<lbrakk> equiv_fpu P s t; equiv_fpu P t u \<rbrakk> \<Longrightarrow> equiv_fpu P s u"
+  by (fastforce simp: equiv_fpu_def equiv_for_def)
+
+lemma equiv_fpu_guard_imp[InfoFlow_IF_assms]:
+  "\<lbrakk> equiv_fpu P s s'; \<And>x. Q x \<Longrightarrow> P x \<rbrakk> \<Longrightarrow> equiv_fpu Q s s'"
+  by (auto simp: equiv_fpu_def equiv_for_def)
+
+lemma equiv_fpu_triv':
+  "\<lbrakk> equiv_fpu P s s'; current_fpu t = current_fpu s; current_fpu t' = current_fpu s';
+     fpu_state (machine_state t) = fpu_state (machine_state s);
+     fpu_state (machine_state t') = fpu_state (machine_state s') \<rbrakk>
+     \<Longrightarrow> equiv_fpu P t t'"
+  by (auto simp: equiv_fpu_def equiv_for_def get_tcb_def hw_fpu_def)
+
+lemma equiv_fpu_triv[InfoFlow_IF_assms]:
+  "\<lbrakk> equiv_fpu P s s'; arch_state t = arch_state s; arch_state t' = arch_state s';
+     machine_state t = machine_state s; machine_state t' = machine_state s' \<rbrakk>
+     \<Longrightarrow> equiv_fpu P t t'"
+  by (fastforce simp: equiv_fpu_triv')
+
+lemma equiv_fpu_machine_state_update[InfoFlow_IF_assms]:
+  "\<lbrakk> equiv_fpu P s s'; identical_fpu_state_updates P s s' ms ms' \<rbrakk>
+     \<Longrightarrow> equiv_fpu P (s\<lparr>machine_state := ms\<rparr>) (s'\<lparr>machine_state := ms'\<rparr>)"
+  by (fastforce simp: equiv_fpu_def equiv_for_def hw_fpu_def
+                      identical_fpu_state_updates_def identical_updates_def
+               split: if_splits)
 
 lemma globals_equiv_refl[InfoFlow_IF_assms]:
   "globals_equiv s s"
@@ -79,9 +167,32 @@ lemma globals_equiv_trans[InfoFlow_IF_assms]:
   unfolding globals_equiv_def arch_globals_equiv_def
   by clarsimp (metis idle_equiv_trans idle_equiv_def)
 
-lemma equiv_asids_guard_imp[InfoFlow_IF_assms]:
-  "\<lbrakk> equiv_asids R s s'; \<And>x. Q x \<Longrightarrow> R x \<rbrakk> \<Longrightarrow> equiv_asids Q s s'"
-  by (auto simp: equiv_asids_def)
+lemma equiv_hypI[InfoFlow_IF_assms]:
+  assumes "\<And>x. P x \<Longrightarrow> equiv_hyp ((=) x) s t"
+  shows "equiv_hyp P s t"
+  using assms by (fastforce simp: equiv_hyp_def equiv_for_def)
+
+lemma equiv_fpuI[InfoFlow_IF_assms]:
+  assumes "\<And>x. P x \<Longrightarrow> equiv_fpu ((=) x) s t"
+  shows "equiv_fpu P s t"
+  using assms by (fastforce simp: equiv_fpu_def equiv_for_def)
+
+end
+
+arch_requalify_consts
+  identical_hyp_state_updates
+  identical_fpu_state_updates
+
+
+global_interpretation InfoFlow_IF_1?: InfoFlow_IF_1 identical_hyp_state_updates identical_fpu_state_updates
+proof goal_cases
+  interpret Arch .
+  case 1 show ?case
+    by (unfold_locales; (fact InfoFlow_IF_assms)?)
+qed
+
+
+context Arch begin arch_global_naming
 
 lemma dmo_loadWord_rev[InfoFlow_IF_assms]:
   "reads_equiv_valid_inv A aag (K (for_each_byte_of_word (aag_can_read aag) p))
@@ -109,10 +220,335 @@ lemma dmo_loadWord_rev[InfoFlow_IF_assms]:
       apply (wp wp_post_taut loadWord_inv | simp)+
   done
 
+definition cur_vcpu_for_2 :: "(obj_ref \<Rightarrow> bool) \<Rightarrow> (obj_ref \<times> bool) option \<rightharpoonup> bool" where
+  "cur_vcpu_for_2 P cv \<equiv> case cv of
+     None \<Rightarrow> None
+   | Some (ptr,b) \<Rightarrow> if P ptr then Some b else None"
+
+locale_abbrev cur_vcpu_for :: "(obj_ref \<Rightarrow> bool) \<Rightarrow> 's state \<rightharpoonup> bool" where
+  "cur_vcpu_for P s \<equiv> cur_vcpu_for_2 P (current_vcpu s)"
+
+lemmas cur_vcpu_for_def = cur_vcpu_for_2_def
+
+lemma hw_vcpu_None[simp]:
+  "hw_vcpu n None vst = None"
+  by (simp add: hw_vcpu_def)
+
+definition equiv_hyp_state :: "nat \<Rightarrow> bool option \<Rightarrow> machine_state \<Rightarrow> machine_state \<Rightarrow> bool" where
+  "equiv_hyp_state n cv ms ms' \<equiv> hw_vcpu n cv (vcpu_state ms) = hw_vcpu n cv (vcpu_state ms')"
+
+definition equiv_fpu_state :: "bool \<Rightarrow> machine_state \<Rightarrow> machine_state \<Rightarrow> bool" where
+  "equiv_fpu_state cf ms ms' \<equiv> hw_fpu cf (fpu_state ms) = hw_fpu cf (fpu_state ms')"
+
+definition no_hyp :: "'a machine_monad \<Rightarrow> bool" where
+  "no_hyp f \<equiv> \<forall>P. \<lbrace>\<lambda>s. P (vcpu_state s)\<rbrace> f \<lbrace>\<lambda>_ s. P (vcpu_state s)\<rbrace>"
+
+definition no_fpu :: "'a machine_monad \<Rightarrow> bool" where
+  "no_fpu f \<equiv> \<forall>P. \<lbrace>\<lambda>s. P (fpu_state s)\<rbrace> f \<lbrace>\<lambda>_ s. P (fpu_state s)\<rbrace>"
+
+lemma equiv_hyp_state_identical_hyp_state_updates:
+  "\<lbrakk> equiv_hyp_state (numlistregs s) (cur_vcpu_for P s) ms ms'; equiv_hyp P s t \<rbrakk>
+     \<Longrightarrow> identical_hyp_state_updates P s t ms ms'"
+  apply (clarsimp simp: equiv_hyp_state_def equiv_for_def identical_hyp_state_updates_def equiv_hyp_def)
+  apply (erule_tac x=x in allE)+
+  apply (drule mp, fastforce)
+  apply (clarsimp simp: cur_vcpu_for_def cur_vcpu_of_def identical_updates_rv_def
+                 split: option.splits if_splits)
+  done
+
+lemma cur_vcpu_for_None:
+  "cur_vcpu_for_2 P None = None"
+  by (clarsimp simp: cur_vcpu_for_def)
+
+lemma cur_vcpu_for_Some:
+  "cur_vcpu_for_2 P (Some (a,b)) = (if P a then Some b else None)"
+  by (clarsimp simp: cur_vcpu_for_def)
+
+lemma cur_vcpu_for_equiv:
+  "\<lbrakk> reads_equiv aag st s; affects_equiv aag l st s \<rbrakk>
+     \<Longrightarrow> cur_vcpu_for (aag_can_read aag or aag_can_affect aag l) st = cur_vcpu_for (aag_can_read aag or aag_can_affect aag l) s"
+  apply (prop_tac "equiv_for (aag_can_read aag or aag_can_affect aag l) cur_vcpu_of st s")
+   apply (simp add: equiv_hyp_def equiv_for_or reads_equiv_def2 affects_equiv_def2 states_equiv_for_def)
+  apply (case_tac "current_vcpu st"; case_tac "current_vcpu s"; clarsimp)
+    apply (clarsimp simp: cur_vcpu_for_None)
+    apply (case_tac "(aag_can_read aag or aag_can_affect aag l) a")
+     prefer 2
+     apply (clarsimp simp: cur_vcpu_for_Some)
+    apply (erule equiv_forE)
+    apply (erule_tac x=a in meta_allE)
+    apply (drule (1) meta_mp)
+    apply (clarsimp simp: cur_vcpu_of_def)
+   apply (clarsimp simp: cur_vcpu_for_None)
+   apply (case_tac "(aag_can_read aag or aag_can_affect aag l) a")
+    prefer 2
+    apply (clarsimp simp: cur_vcpu_for_Some)
+   apply (erule equiv_forE)
+   apply (erule_tac x=a in meta_allE)
+   apply (drule (1) meta_mp)
+   apply (clarsimp simp: cur_vcpu_of_def)
+  apply (case_tac "(aag_can_read aag or aag_can_affect aag l) a"; case_tac "(aag_can_read aag or aag_can_affect aag l) aa")
+     apply (erule equiv_forE)
+     apply (erule_tac x=a in meta_allE)
+     apply (drule (1) meta_mp)
+     apply (clarsimp simp: cur_vcpu_of_def split: if_splits)
+    apply (erule equiv_forE)
+    apply (erule_tac x=a in meta_allE)
+    apply (drule (1) meta_mp)
+    apply (clarsimp simp: cur_vcpu_of_def split: if_splits)
+   apply (erule equiv_forE)
+   apply (erule_tac x=aa in meta_allE)
+   apply (drule (1) meta_mp)
+   apply (clarsimp simp: cur_vcpu_of_def split: if_splits)
+  apply (clarsimp simp: cur_vcpu_for_Some)
+  done
+
+lemma aequiv_get_tcb_eq'[intro]:
+  "\<lbrakk> affects_equiv aag l s t; aag_can_affect aag l thread \<rbrakk>
+     \<Longrightarrow> get_tcb thread s = get_tcb thread t"
+  by (auto simp: affects_equiv_def2 get_tcb_def elim: states_equiv_forE_kheap)
+
+definition cur_fpu_for :: "(obj_ref \<Rightarrow> bool) \<Rightarrow> 's state \<Rightarrow> bool" where
+  "cur_fpu_for P s \<equiv> \<exists>ptr. P ptr \<and> is_arch_cur_fpu ptr s"
+
+lemma equiv_fpu_cur_fpu_for:
+  "equiv_fpu P st s \<Longrightarrow> cur_fpu_for P st = cur_fpu_for P s"
+  apply (clarsimp simp: equiv_fpu_def equiv_for_def cur_fpu_for_def)
+  apply (rule iffI; erule ex_forward; erule_tac x=ptr in allE; clarsimp simp: hw_fpu_def split: if_splits)
+  done
+
+lemma cur_fpu_for_equiv:
+  "\<lbrakk> reads_equiv aag st s; affects_equiv aag l st s \<rbrakk>
+     \<Longrightarrow> cur_fpu_for (aag_can_read aag or aag_can_affect aag l) st =
+         cur_fpu_for (aag_can_read aag or aag_can_affect aag l) s"
+  apply (prop_tac "equiv_fpu (aag_can_read aag or aag_can_affect aag l) st s")
+   apply (clarsimp simp: reads_equiv_def2 affects_equiv_def2 states_equiv_for_def equiv_fpu_def equiv_for_def)
+  apply (simp add: equiv_fpu_cur_fpu_for)
+  done
+
+lemma equiv_fpu_state_identical_fpu_state_updates:
+  "\<lbrakk> equiv_fpu_state (cur_fpu_for P s) ms ms'; equiv_fpu P s t \<rbrakk>
+     \<Longrightarrow> identical_fpu_state_updates P s t ms ms'"
+  unfolding identical_fpu_state_updates_def
+  apply (clarsimp simp: identical_fpu_state_updates_def identical_updates_def)
+  apply (clarsimp simp: equiv_fpu_state_def equiv_for_def equiv_fpu_def)
+  apply (erule_tac x=x in allE, clarsimp)
+  apply (auto simp: cur_fpu_for_def hw_fpu_def get_tcb_def identical_updates_rv_def split: if_splits option.splits kernel_object.splits)
+  done
+
+definition numlistregs_for :: "(obj_ref \<Rightarrow> bool) \<Rightarrow> 's state \<Rightarrow> nat" where
+  "numlistregs_for P s \<equiv> if \<exists>p. P p then numlistregs s else undefined"
+
+lemma numlistregs_for_equiv:
+  "\<lbrakk> reads_equiv aag st s; affects_equiv aag l st s \<rbrakk>
+     \<Longrightarrow> numlistregs_for (aag_can_read aag or aag_can_affect aag l) st = numlistregs_for (aag_can_read aag or aag_can_affect aag l) s"
+  by (auto simp: reads_equiv_def2 affects_equiv_def2 states_equiv_for_def equiv_hyp_def equiv_for_def numlistregs_for_def)
+
+lemma equiv_hyp_state_sym:
+  "equiv_hyp_state n cv ms' ms \<Longrightarrow> equiv_hyp_state n cv ms ms'"
+  by (simp add: equiv_hyp_state_def)
+
+lemma equiv_fpu_state_sym:
+  "equiv_fpu_state cf ms' ms \<Longrightarrow> equiv_fpu_state cf ms ms'"
+  by (simp add: equiv_fpu_state_def)
+
+lemma spec_equiv_valid_add_inv:
+  assumes "spec_equiv_valid st I A B (P and I st) f"
+  and "\<And>s. I s s"
+  shows "spec_equiv_valid st I A B P f"
+  using assms by (fastforce simp: spec_equiv_valid_def equiv_valid_2_def)
+
+lemma spec_equiv_valid_add_A:
+  assumes "spec_equiv_valid st I A B (P and A st) f"
+  and "\<And>s. A s s"
+  shows "spec_equiv_valid st I A B P f"
+  using assms by (fastforce simp: spec_equiv_valid_def equiv_valid_2_def)
+
+lemma do_machine_op_reads_respects'':
+  assumes equiv_dmo:
+   "\<And>n cv cf. equiv_valid_inv (equiv_irq_state and equiv_machine_state (aag_can_read aag)
+                                                and equiv_hyp_state n cv and equiv_fpu_state cf)
+                               (equiv_machine_state (aag_can_affect aag l)) (Q n cv cf) f"
+  assumes guard:
+    "\<And>s. P s \<Longrightarrow> Q (numlistregs_for (aag_can_read aag or aag_can_affect aag l) s)
+                    (cur_vcpu_for (aag_can_read aag or aag_can_affect aag l) s)
+                    (cur_fpu_for (aag_can_read aag or aag_can_affect aag l) s)
+                    (machine_state s)"
+    (is "\<And>s. P s \<Longrightarrow> Q (?nlf s) (?cvf s) (?cff s) (machine_state s)")
+  shows
+    "reads_respects aag l P (do_machine_op f)"
+  apply (rule use_spec_ev)
+  apply (rule spec_equiv_valid_add_inv)
+   prefer 2
+   apply (simp add: reads_equiv_refl)
+  apply (rule spec_equiv_valid_add_A)
+   prefer 2
+   apply (simp add: affects_equiv_refl)
+  apply (unfold do_machine_op_def spec_equiv_valid_def)
+  supply equiv_for_disj[simp]
+  apply (rule equiv_valid_2_guard_imp)
+    apply (rule_tac R'="\<lambda>rv rv'. equiv_machine_state (aag_can_read_or_affect aag l) rv rv' \<and>
+                                 equiv_irq_state rv rv' \<and>
+                                 equiv_hyp_state (?nlf st) (?cvf st) rv rv' \<and>
+                                 equiv_fpu_state (?cff st) rv rv'"
+                and Q="\<lambda>r s. st = s \<and> Q (?nlf st) (?cvf st) (?cff st) r"
+                and Q'="\<lambda>r s. Q (?nlf st) (?cvf st)
+                                (?cff st) r"
+                and P="(=) st" and P'="\<top>" in equiv_valid_2_bind)
+       apply (rule gen_asm_ev2_l[simplified K_def pred_conj_def])
+       apply (rule gen_asm_ev2_r')
+       apply (rule_tac R'="\<lambda>(r, ms') (r', ms''). r = r'
+                                               \<and> equiv_machine_state (aag_can_read_or_affect aag l) ms' ms''
+                                               \<and> equiv_irq_state ms' ms''
+                                               \<and> equiv_hyp_state (?nlf st) (?cvf st) ms' ms''
+                                               \<and> equiv_fpu_state (?cff st) ms' ms''"
+                   and Q="\<lambda>r s. s = st"
+                   and Q'="\<top>\<top>"
+                   and P="\<top>" and P'="\<top>" in equiv_valid_2_bind_pre)
+            apply (clarsimp simp: modify_def get_def put_def bind_def return_def equiv_valid_2_def)
+            apply (rule conjI)
+             apply (rule reads_equiv_machine_state_update; clarsimp?)
+              apply (rule equiv_hyp_state_identical_hyp_state_updates)
+               apply (clarsimp simp: equiv_hyp_state_def cur_vcpu_for_def numlistregs_for_def
+                              split: option.splits if_splits)
+              apply (erule reads_equivE, clarsimp simp: equiv_hyp_def)
+             apply (rule equiv_fpu_state_identical_fpu_state_updates)
+              apply (fastforce simp: equiv_fpu_state_def cur_fpu_for_def hw_fpu_def
+                              split: option.splits if_splits)
+             apply (erule reads_equivE, clarsimp simp: equiv_fpu_def)
+            apply (rule affects_equiv_machine_state_update; clarsimp?)
+             apply (rule equiv_hyp_state_identical_hyp_state_updates)
+              apply (clarsimp simp: equiv_hyp_state_def cur_vcpu_for_def numlistregs_for_def
+                             split: option.splits if_splits)
+             apply (erule affects_equivE, clarsimp simp: equiv_hyp_def)
+            apply (rule equiv_fpu_state_identical_fpu_state_updates)
+             apply (fastforce simp: equiv_fpu_state_def cur_fpu_for_def hw_fpu_def
+                             split: option.splits if_splits)
+            apply (erule affects_equivE, clarsimp simp: equiv_fpu_def)
+           apply (insert equiv_dmo)[1]
+           apply (clarsimp simp: select_f_def equiv_valid_2_def equiv_valid_def2 equiv_for_or
+                           simp: split_def split: prod.splits simp: equiv_for_def)[1]
+           apply (erule_tac x="?nlf st" in meta_allE)
+           apply (erule_tac x="?cvf st" in meta_allE)
+           apply (erule_tac x="?cff st" in meta_allE)
+           apply (drule_tac x=rv in spec, drule_tac x=rv' in spec)
+           apply clarsimp
+           apply (drule (1) bspec)+
+           apply clarsimp
+          apply wp
+         apply wp
+        apply clarsimp
+       apply clarsimp
+      apply (clarsimp simp: equiv_valid_2_def in_monad)
+      apply (intro conjI)
+            apply (fastforce elim: reads_equivE affects_equivE equiv_forE intro: equiv_forI)
+           apply (fastforce elim: reads_equivE affects_equivE equiv_forE intro: equiv_forI)
+          apply (fastforce elim: reads_equivE affects_equivE equiv_forE intro: equiv_forI)
+         apply (fastforce elim: reads_equivE affects_equivE equiv_forE intro: equiv_forI)
+        apply (fastforce elim: reads_equivE affects_equivE equiv_forE intro: equiv_forI)
+       apply (frule (1) cur_vcpu_for_equiv)
+       apply (clarsimp simp: equiv_hyp_state_def)
+       apply (prop_tac "equiv_for (aag_can_read aag or aag_can_affect aag l) (K \<circ> numlistregs) st t")
+        apply (simp add: equiv_hyp_def equiv_for_or reads_equiv_def2 affects_equiv_def2 states_equiv_for_def)
+       apply (prop_tac "equiv_for (aag_can_read aag or aag_can_affect aag l) hw_vcpu_of st t")
+        apply (simp add: equiv_hyp_def equiv_for_or reads_equiv_def2 affects_equiv_def2 states_equiv_for_def)
+       apply (case_tac "cur_vcpu_for (aag_can_read aag or aag_can_affect aag l) t"; clarsimp)
+       apply (clarsimp simp: cur_vcpu_for_def split: option.splits if_splits)
+       apply (erule equiv_forE)+
+       apply (erule_tac x=aa in meta_allE, clarsimp)+
+       apply (clarsimp simp: cur_vcpu_of_def hw_vcpu_def numlistregs_for_def split: if_splits)
+      apply (frule (1) cur_fpu_for_equiv)
+      apply (clarsimp simp: equiv_fpu_state_def)
+      apply (prop_tac "equiv_for ((aag_can_read aag or aag_can_affect aag l)) hw_fpu_of st t")
+       apply (simp add: equiv_fpu_def equiv_for_or reads_equiv_def2 affects_equiv_def2 states_equiv_for_def)
+      apply (fastforce simp: equiv_for_def hw_fpu_def cur_fpu_for_def split: if_splits)
+     apply (wp | simp add: guard)+
+  using guard cur_fpu_for_equiv cur_vcpu_for_equiv numlistregs_for_equiv apply fastforce
+  done
+
+lemma do_machine_op_reads_respects'[InfoFlow_IF_assms]:
+  assumes equiv_dmo:
+    "equiv_valid_inv (equiv_machine_state (aag_can_read aag) and equiv_irq_state)
+                    (equiv_machine_state (aag_can_affect aag l)) Q f"
+  assumes guard: "\<And>s. P s \<Longrightarrow> Q (machine_state s)"
+  assumes no_hyp: "no_hyp f"
+  assumes no_fpu: "no_fpu f"
+  shows "reads_respects aag l P (do_machine_op f)"
+  apply (rule do_machine_op_reads_respects''[where Q="\<lambda>_ _ _. Q"])
+   apply (insert equiv_dmo no_hyp no_fpu)
+   apply (clarsimp simp: equiv_valid_2_def equiv_valid_def2 equiv_for_or no_hyp_def no_fpu_def
+                         equiv_for_def split_def)
+   apply (rename_tac rv st rv' st')
+   apply (drule_tac x=s in spec, drule_tac x=t in spec)
+   apply clarsimp
+   apply (drule (1) bspec)+
+   apply clarsimp
+   apply (rule conjI)
+    apply (clarsimp simp: equiv_hyp_state_def)
+    apply (erule use_valid, erule spec)+
+    apply clarsimp
+   apply (clarsimp simp: equiv_fpu_state_def)
+   apply (erule use_valid, erule spec)+
+   apply clarsimp
+  apply (simp add: guard)
+  done
+
+lemma equiv_hyp_state_upds[simp]:
+  "\<And>f. equiv_hyp_state n cv ms (underlying_memory_update f ms') = equiv_hyp_state n cv ms ms'"
+  "\<And>f. equiv_hyp_state n cv (underlying_memory_update f ms) ms' = equiv_hyp_state n cv ms ms'"
+  "\<And>f. equiv_hyp_state n cv ms (device_state_update f ms') = equiv_hyp_state n cv ms ms'"
+  "\<And>f. equiv_hyp_state n cv (device_state_update f ms) ms' = equiv_hyp_state n cv ms ms'"
+  "\<And>f. equiv_hyp_state n cv ms (machine_state_rest_update f ms') = equiv_hyp_state n cv ms ms'"
+  "\<And>f. equiv_hyp_state n cv (machine_state_rest_update f ms) ms' = equiv_hyp_state n cv ms ms'"
+  by (auto simp: equiv_hyp_state_def)
+
+lemma equiv_fpu_state_upds[simp]:
+  "\<And>f. equiv_fpu_state cf ms (underlying_memory_update f ms') = equiv_fpu_state cf ms ms'"
+  "\<And>f. equiv_fpu_state cf (underlying_memory_update f ms) ms' = equiv_fpu_state cf ms ms'"
+  "\<And>f. equiv_fpu_state cf ms (device_state_update f ms') = equiv_fpu_state cf ms ms'"
+  "\<And>f. equiv_fpu_state cf (device_state_update f ms) ms' = equiv_fpu_state cf ms ms'"
+  "\<And>f. equiv_fpu_state cf ms (machine_state_rest_update f ms') = equiv_fpu_state cf ms ms'"
+  "\<And>f. equiv_fpu_state cf (machine_state_rest_update f ms) ms' = equiv_fpu_state cf ms ms'"
+  by (auto simp: equiv_fpu_state_def)
+
+lemma no_hyp_bind:
+  "\<lbrakk> no_hyp f; \<And>rv. no_hyp (g rv) \<rbrakk> \<Longrightarrow> no_hyp (f >>= g)"
+  unfolding no_hyp_def
+  by (wpsimp, blast+)
+
+lemma no_fpu_bind:
+  "\<lbrakk> no_fpu f; \<And>rv. no_fpu (g rv) \<rbrakk> \<Longrightarrow> no_fpu (f >>= g)"
+  unfolding no_fpu_def
+  by (wpsimp, blast+)
+
+lemma equiv_hyp_state_lift[wp]:
+  assumes "\<And>P. f \<lbrace>\<lambda>s. P (vcpu_state s)\<rbrace>"
+  shows "f \<lbrace>equiv_hyp_state n cv st\<rbrace>"
+  unfolding equiv_hyp_state_def
+  by (wp assms)
+
+lemma equiv_fpu_state_lift[wp]:
+  assumes "\<And>P. f \<lbrace>\<lambda>s. P (fpu_state s)\<rbrace>"
+  shows "f \<lbrace>equiv_fpu_state cf st\<rbrace>"
+  unfolding equiv_fpu_state_def
+  by (wp assms)
+
+lemma no_hyp_lift[wp]:
+  assumes "\<And>P. f \<lbrace>\<lambda>s. P (vcpu_state s)\<rbrace>"
+  shows "no_hyp f"
+  using assms by (simp add: no_hyp_def)
+
+lemma no_fpu_lift[wp]:
+  assumes "\<And>P. f \<lbrace>\<lambda>s. P (fpu_state s)\<rbrace>"
+  shows "no_fpu f"
+  using assms by (simp add: no_fpu_def)
+
 end
 
+arch_requalify_consts
+  no_hyp no_fpu
 
-global_interpretation InfoFlow_IF_1?: InfoFlow_IF_1
+
+global_interpretation InfoFlow_IF_2?: InfoFlow_IF_2 identical_hyp_state_updates identical_fpu_state_updates no_hyp no_fpu
 proof goal_cases
   interpret Arch .
   case 1 show ?case
